Validator/Expr/IfExpr.lean
@@ -12,17 +12,17 @@ abbrev IfExprs n α l := List.Vector (IfExpr n α) l
 
 namespace IfExpr
 
-def eval {α: Type} [DecidableEq α] (g: Grammar n α Pred) (ifExpr: IfExpr n α) (t: α): Rule n α Pred :=
+def eval {α: Type} [DecidableEq α] (g: Grammar n (Pred α)) (ifExpr: IfExpr n α) (t: α): Rule n (Pred α) :=
   match ifExpr with
   | IfExpr.mk cnd thn =>
     if Pred.eval cnd t
     then g.lookup thn
     else Regex.emptyset
 
-def evals {α: Type} {n: Nat} [DecidableEq α] (g: Grammar n α Pred) (ifExprs: IfExprs n α l) (t: α): Rules n α Pred l :=
+def evals {α: Type} {n: Nat} [DecidableEq α] (g: Grammar n (Pred α)) (ifExprs: IfExprs n α l) (t: α): Rules n (Pred α) l :=
   List.Vector.map (fun x => eval g x t) ifExprs
 
-theorem evals_nil_is_nil {α: Type} {n: Nat} [DecidableEq α] (g: Grammar n α Pred) (a: α):
+theorem evals_nil_is_nil {α: Type} {n: Nat} [DecidableEq α] (g: Grammar n (Pred α)) (a: α):
   evals g (n := n) List.Vector.nil a = List.Vector.nil := by
   unfold evals
   simp
