Validator/Learning/ImperativeBasic.lean
@@ -16,13 +16,13 @@ import Validator.Learning.ImperativeLeave
 namespace ImperativeBasic
 
 -- foldLoop is a more readable version of List.foldlM for imperative programmers:
-private def foldLoop (deriv: List (Rule μ α Pred) -> Hedge.Node α -> List (Rule μ α Pred)) (start: List (Rule μ α Pred)) (hedge: Hedge α): Id (List (Rule μ α Pred)) := do
+private def foldLoop (deriv: List (Rule μ (Pred α)) -> Hedge.Node α -> List (Rule μ (Pred α))) (start: List (Rule μ (Pred α))) (hedge: Hedge α): Id (List (Rule μ (Pred α))) := do
   let mut res := start
   for tree in hedge do
     res := deriv res tree
   return res
 
-def derive [DecidableEq α] (g: Grammar μ α Pred) (xs: List (Rule μ α Pred)) (tree: Hedge.Node α): List (Rule μ α Pred) :=
+def derive [DecidableEq α] (g: Grammar μ (Pred α)) (xs: List (Rule μ (Pred α))) (tree: Hedge.Node α): List (Rule μ (Pred α)) :=
   -- If all expressions are unescapable, then simply return without look at the input tree.
   -- An example of an unescapable expression is emptyset, since its derivative is always emptyset, no matter the input.
   if List.all xs Regex.unescapable
@@ -34,28 +34,28 @@ def derive [DecidableEq α] (g: Grammar μ α Pred) (xs: List (Rule μ α Pred))
       -- enters is one of our two new memoizable functions.
       let ifexprs: List (IfExpr μ α) := Enter.deriveEnter_list xs
       -- childxs = expressions to evaluate on children.
-      let childxs: List (Rule μ α Pred) := List.map (fun x => IfExpr.eval g x label) ifexprs
+      let childxs: List (Rule μ (Pred α)) := List.map (fun x => IfExpr.eval g x label) ifexprs
       -- dchildxs = derivatives of children. The ' is for the exception it is wrapped in.
       -- see foldLoop for an explanation of what List.foldM does.
-      let dchildxs: List (Rule μ α Pred) := List.foldl (derive g) childxs children
+      let dchildxs: List (Rule μ (Pred α)) := List.foldl (derive g) childxs children
       -- dxs = derivatives of xs. The ' is for the exception it is wrapped in.
       -- leaves is the other one of our two new memoizable functions.
-      let dxs: List (Rule μ α Pred) := ImperativeLeave.deriveLeave xs (List.map Regex.nullable dchildxs)
+      let dxs: List (Rule μ (Pred α)) := ImperativeLeave.deriveLeave xs (List.map Regex.nullable dchildxs)
       dxs
 
-def derivs [DecidableEq α] (g: Grammar μ α Pred) (x: Rule μ α Pred) (hedge: Hedge α): Except String (Rule μ α Pred) :=
+def derivs [DecidableEq α] (g: Grammar μ (Pred α)) (x: Rule μ (Pred α)) (hedge: Hedge α): Except String (Rule μ (Pred α)) :=
   -- see foldLoop for an explanation of what List.foldM does.
   let dxs := List.foldl (derive g) [x] hedge
   match dxs with
   | [dx] => Except.ok dx
   | _ => Except.error "expected one expression"
 
-def validate [DecidableEq α] (g: Grammar μ α Pred) (x: Rule μ α Pred) (hedge: Hedge α): Except String Bool :=
+def validate [DecidableEq α] (g: Grammar μ (Pred α)) (x: Rule μ (Pred α)) (hedge: Hedge α): Except String Bool :=
   match derivs g x hedge with
   | Except.error err => Except.error err
   | Except.ok x' => Except.ok (Rule.nullable x')
 
-def run [DecidableEq α] (g: Grammar μ α Pred) (t: Hedge.Node α): Except String Bool :=
+def run [DecidableEq α] (g: Grammar μ (Pred α)) (t: Hedge.Node α): Except String Bool :=
   validate g g.start [t]
 
 -- Tests
