Validator/Derive/Enter.lean
@@ -7,7 +7,7 @@ import Validator.Expr.Symbol
 
 namespace Enter
 
-def deriveEnter (xs: Rules n α Pred l): IfExprs n α (Symbol.nums xs) :=
+def deriveEnter (xs: Rules n (Pred α) l): IfExprs n α (Symbol.nums xs) :=
   List.Vector.map
     (fun (pred, ref) => IfExpr.mk pred ref)
     (Symbol.Symbols.cast
@@ -16,7 +16,7 @@ def deriveEnter (xs: Rules n α Pred l): IfExprs n α (Symbol.nums xs) :=
     )
 
 class DeriveEnter (m: Type -> Type u) (n: Nat) (α: outParam Type) where
-  deriveEnter {l: Nat} (xs: Rules n α Pred l): m (IfExprs n α (Symbol.nums xs))
+  deriveEnter {l: Nat} (xs: Rules n (Pred α) l): m (IfExprs n α (Symbol.nums xs))
 
-def deriveEnter_list (xs: List (Rule n α Pred)): List (IfExpr n α) :=
+def deriveEnter_list (xs: List (Rule n (Pred α))): List (IfExpr n α) :=
   List.map (fun (pred, ref) => IfExpr.mk pred ref) (Symbol.extracts_list xs []).2
