Validator/Validator/Inst/TreeParserIO.lean
@@ -64,7 +64,7 @@ instance [DecidableEq α] [Hashable α]: MemEnter (Impl μ α) μ α where
 
 -- This should just follow from the instance declared in MemEnter, but we spell it out just in case.
 instance [DecidableEq α] [Hashable α]: Enter.DeriveEnter (Impl μ α) μ α where
-  deriveEnter {ν: Nat} (xs: Rules μ α Pred ν): Impl μ α (IfExprs μ α (Symbol.nums xs)) := MemEnter.deriveEnter xs
+  deriveEnter {ν: Nat} (xs: Rules μ (Pred α) ν): Impl μ α (IfExprs μ α (Symbol.nums xs)) := MemEnter.deriveEnter xs
 
 instance [DecidableEq α] [Hashable α]: MemLeave (Impl μ α) μ α where
   getLeave : Impl μ α (MemLeave.LeaveMap μ α) := do
@@ -77,7 +77,7 @@ instance [DecidableEq α] [Hashable α]: MemLeave (Impl μ α) μ α where
 
 -- This should just follow from the instance declared in MemLeave, but we spell it out just in case.
 instance [DecidableEq α] [Hashable α]: Leave.DeriveLeaveM (Impl μ α) μ α where
-  deriveLeaveM {ν: Nat} (xs: Rules μ α Pred ν) (ns: List.Vector Bool (Symbol.nums xs)): Impl μ α (Rules μ α Pred ν) := MemLeave.deriveLeaveM xs ns
+  deriveLeaveM {ν: Nat} (xs: Rules μ (Pred α) ν) (ns: List.Vector Bool (Symbol.nums xs)): Impl μ α (Rules μ (Pred α) ν) := MemLeave.deriveLeaveM xs ns
 
 instance [DecidableEq α] [Hashable α]: ValidateM (Impl μ α) μ α where
   -- all instances have been created, so no implementations are required here
